Implemented Spec, Message, and working on Host

project02/AtomicKVSpec.t.dfy
@@ -28,16 +28,45 @@ module AtomicKVSpec {
   // Be sure to check out IMapHelpers.t.dfy. It's helpful.
   ghost predicate Init(c: Constants, v: Variables) {
   /*{*/
-    && v.mp == ZeroMap()
+    && v.mp == ZeroMap() 
   /*}*/
   }
 
   /*{*/
+  // Model the Get event to accept a key and return a value
+  ghost predicate GetEvt(v: Variables, v': Variables, key: int, value: int) 
+  {
+    && IsFull(v.mp)
+    && value == v.mp[key]
+    && v' == v
+  }
+
+  // Model the Put event to update the key's value 
+  ghost predicate PutEvt(v: Variables, v': Variables, key: int, value: int) 
+  {
+    && IsFull(v.mp)
+    // v' is updated such that v's map at key value is now set to "value"
+    // First, remove the original key value from v.mp
+    && var keyset: iset<int> := iset {key};
+    var rm_mp := MapRemove(v.mp, keyset);
+
+    // Second, create a temp imap with key, value
+    var t := imap[key := value];
+
+    // Last, union the maps and prefer the original map (to take in the new key, value)
+    var tmp := IMapUnionPreferLeft(v.mp, t);
+    && v' == v.(mp := tmp)
+  }
+
   /*}*/
 
 ghost predicate NextStep(c: Constants, v: Variables, v': Variables, event: Event) {
   /*{*/
-    true // Replace me
+    match event {
+      case Get(key, value) => GetEvt(v, v', key, value)
+      case Put(key, value) => PutEvt(v, v', key, value)
+      case NoOp => v' == v
+    }
   /*}*/
 }
 
